\section{Construction of coherent states for bosons, and its properties}\label{unc:order_boson}

Pages 18-26 in lecture notes.

\subsection{Construction}
The definition of a coherent boson state $\ket{\phi}$ is stated in \eqref{eq:def_boson_coherent_state}. We make an ansatz -- a qualified guess -- that $\ket{\phi}$ can be created as
\begin{equation}
\label{eq:construction_coherent_boson}
\ket{\phi} = \e^{\sum_\mu\varphi_\mu a_\mu^\dagger}\ket{0}.
\end{equation}

We claim that 
\begin{equation}
\label{unc:indices}
a_\mu\e^{\sum_\nu\varphi_\nu a_\nu^\dagger}\ket{0} = \varphi_\mu\e^{\sum_\nu\varphi_\nu a_\nu^\dagger}\ket{0}
\end{equation} % TODO: CHECK THIS

\begin{proof}
\label{unc:proof}
\begin{equation*}
a\sum_{n=0}\frac{\left(\varphi a^\dagger\right)^n}{n!}\ket{0} = a\sum_{n=1} \frac{\varphi^n}{n!}\left(a^\dagger\right)^n\ket{0}.
\end{equation*}
Note that $\left(a^\dagger\right)^na\ket{0} = 0$, and so we wish to ``commute $a$ through''.

\begin{align*}
\comm{a}{f\left(a^\dagger\right)} &= \sum_{n=1}c_n\comm{a}{\left(a^\dagger\right)^n} \\
&= \sum_{n=1}nc_n\left(a^\dagger\right)^{n-1}\\
f\left(a^\dagger\right) &= \sum_{n=0}^\infty c_n\left(a^\dagger\right)^n \\
&\implies \comm{a}{f\left(a^\dagger\right)} = \pdv{a^\dagger}f\left(a^\dagger\right).
\end{align*}

More generally:

\begin{align*}
\comm{g(a)}{f(a^\dagger)} &= g\left(\pdv{a^\dagger}\right)f\left(a^\dagger\right)\\
\comm{a}{\left(a^\dagger\right)^n} &= n\left(a^\dagger\right)^{n-1} \\
\comm{\left(a\right)^m}{\left(a^\dagger\right)^n} &= \frac{n!}{(n-m)!}\left(a^\dagger\right)^{n-m} \\
\acomm{c}{f\left(c^\dagger\right)} &= \pdv{c^\dagger}f\left(c^\dagger\right) \\
\acomm{g(c)}{f(c^\dagger)} &= g\left(\pdv{c^\dagger}\right)f\left(c^\dagger\right)
\end{align*}

To find out what the commutator $\comm{a}{\left(a^\dagger\right)^n}$ is, we use that 
\begin{equation}
\comm{A}{BC} = \comm{A}{B}C + B\comm{A}{C}, 
\end{equation}
with $A =a, B = a^\dagger, C = \left(a^\dagger\right)^{n-1}$ to get

\begin{align*}
\comm{a}{\left(a^\dagger\right)^n} &= \left(a^\dagger\right)^{n-1} + a^\dagger\comm{a}{\left(a^\dagger\right)^{n-1}} \\
&= a\left(a^\dagger\right)^{n-1} \\
\implies a\left(a^\dagger\right)^{n}\ket{0} &= n\left(a^\dagger\right)^{n-1}\ket{0}\\
\implies a\e^{\varphi a^\dagger}\ket{0} &= \sum_{n=1}^\infty\frac{\varphi^nn\left(a^\dagger\right)^{n-1}}{n!}\ket{0} \\
&= \varphi\sum_{n=1}^\infty\frac{\left(\varphi a^\dagger\right)^{n-1}}{(n-1)!}\ket{0}\\ &= \varphi\e^{\varphi a^\dagger}\ket{0}.
\end{align*}
\end{proof}

Then, for more modes (quantum numbers), we get
\begin{equation}
\ket{\phi} = \e^{\sum_\mu\varphi_\mu a_\mu^\dagger}\ket{0}
\end{equation}
with the $\varphi_\mu$'s satisfying
\begin{equation}
a_\mu\ket{\phi} = \varphi_\mu\ket{\phi}.
\end{equation}
Coherent states: ``difficult to destroy''.

We also could have done this in a more direct way:
Assume
\begin{equation}
\ket{\phi} = \prod_\mu f_\mu\left(\varphi, a_\mu^\dagger\right)\ket{0}
\end{equation}
with 
\begin{equation}
a_\mu =\varphi_\mu\ket{\phi}.
\end{equation}

Then, we need that 
\begin{equation}
a_\mu f_\mu\left(\varphi, a_\mu^\dagger\right)\ket{0} = \varphi_\mu f_\mu\left(\varphi, a_\mu^\dagger\right)\ket{0},
\end{equation}

but

\begin{align}
a_\mu f_\mu \ket{0} &= \comm{a_\mu}{f_\mu}\ket{0}\\
&\implies \pdv{a_\mu^\dagger} f_\mu = \varphi_\mu f_\mu \\
\implies \frac{\dd{f_\mu}}{{f_\mu}} &= \varphi_\mu \dd{a_\mu^\dagger} \\
\ln f_\mu &= \varphi_\mu a_\mu^\dagger \\
f_\mu &= \e^{\varphi_\mu a_\mu^\dagger}.
\end{align}

\subsection{Properties}
We will now look at some of the properties of coherent bosonic states. 
\begin{align}
a_\mu^\dagger\ket{\phi} &= a_\mu^\dagger\e^{\sum_\mu\varphi_\nu a_\nu^\dagger}\ket{0}\\
&= \pdv{\varphi_\mu}\ket{\phi}
\end{align}

\begin{align}
\bra{\phi} &= \bra{0}\e^{\sum_\mu \varphi_\mu^*a_\mu} \implies\\
\bra{\phi}a_\mu &= \pdv{\varphi_\mu^*}\bra{\phi}
\end{align}

The overlap of two coherent bosonic states are
\begin{equation}
\braket{\phi}{\sigma} = \mel{0}{\e^{\sum_\mu\varphi_\mu^*a_\mu}\e^{\sum_\nu\sigma_\nu a_\nu^\dagger}}{0}.
\end{equation}

Now define 
\begin{align*}
A &= \sum_\mu\varphi_\mu^*a_\mu \\
B &= \sum_\nu\sigma_\nu a_\nu
\end{align*}

such that 
\begin{equation}
\braket{\phi}{\sigma} = \mel{0}{\e^{A}\e^{B}}{0}.
\end{equation}

We see that 
\begin{equation}
\mel{0}{\e^{B}\e^{A}}{0} = 1.
\end{equation}

Baker-Hausdorff:
\begin{align}
e^{A+B} &=\e^{A}\e^{B}\e^{-\frac{1}{2}\comm{A}{B}} \\
		&= \e^{B}\e^{A}\e^{-\frac{1}{2}\comm{B}{A}},
\end{align}

where $\comm{A}{B}$ commutes with $A, B$.
\begin{align}
\implies \e^A\e^B &= \e^B\e^A\e^{\comm{A}{B}} \\
\comm{A}{B} &= \sum_{\mu,\nu}\varphi_\mu^*\sigma_\nu\underbrace{\comm{a_\mu}{a_\nu^\dagger}}_{\delta_{\mu\nu}} \\
	&= \sum_\mu\varphi_\mu^*\sigma_\mu \\
	\implies& \\
	 \braket{\phi}{\sigma} &= \e^{\sum_\mu\varphi_\mu^*\sigma_\mu}\underbrace{\mel{0}{\e^B\e^A}{0}}_{=1}\\
	 &= \e^{\sum_\mu\varphi_\mu^*\sigma_\mu},
\end{align}
the states are not orthogonal!

For the normalization of \(\ket{\phi}\) we have
\begin{align}
\braket{\phi} &= \e^{\sum_\mu\varphi_\mu^*\varphi_\mu} \\
	&= \e^{\ev{N}}.
\end{align}
\(\ev{N}\) is the average number of particles in the state \(\ket{\phi}\)

\begin{align}\label{unc:expvalN}
\frac{\ev{\sum_\mu a_\mu^\dagger a_\mu}{\phi}}{\braket{\phi}} &= \ev{N} \\
&= \sum_\mu \varphi_\mu^*\varphi_\mu
\end{align}

\begin{align}
\ev{\left(\Delta N \right)^2} &= \frac{1}{\braket{\phi}}\left[ \ev{\hat{N}^2}{\phi} - \left( \ev{\hat{N}}{\phi}\right)^2\right] \\
&= \frac{1}{\braket{\phi}}\left[\ev{\sum_{\mu, \nu}a_\mu^\dagger a_\mu a_\nu^\dagger a_\nu}{\phi} - \left(\sum_\mu\varphi_\mu^*\varphi_\mu\right)^2\right]\\
\label{unc:expvalN2}
&= \sum_\mu\varphi_\mu^*\varphi_\mu = N.
\end{align}

\subsubsection{Coherent states for a one-bosonic oscillator}

Following the construction from \eqref{eq:construction_coherent_boson}, we have
\begin{align}
\ket{z} &= \e^{za^\dagger}\ket 0 \\
&= \sum_{n=0}^\infty \frac{z^n\left(a^\dagger\right)^n}{n!}\ket{0} = \sum_n \frac{z^n}{\sqrt{n!}}\frac{\left(a^\dagger\right)}{\sqrt{n!}}\ket 0 \\
&= \sum_n\frac{z^n}{\sqrt{n!}}\ket n
\end{align}

\begin{align}
\label{eq:completeness_coherent_boson}
&\frac{1}{2\pi i}\int\dd z \dd{z^*}\e^{-z^*z}\dyad z \\
&= \frac{1}{2\pi i}\int \dd z \dd{z^*}\e^{-zz^*}\sum_{n,m}\frac{z^n}{\sqrt{n!}}\frac{\left(z^*\right)^m}{\sqrt{m!}}\dyad m \\
&= \frac{1}{2\pi i}\sum_{n, m}\frac{1}{\sqrt{n!m!}}\dyad{n}{m}\int\dd z \dd{z^*}\e^{-zz^*}z^n\left(z^*\right)^m \\
&= \frac{1}{\pi}\sum_{n, m}\frac{1}{\sqrt{n!m!}}\dyad{n}{m}\int \dd{x}\dd{y} \e^{-\left(x^2 + y^2\right)}\left(x+iy\right)^n)\left(x-iy\right)^m. \label{eq:coherent_state_integral}
\end{align}
Now, the integral in \eqref{eq:coherent_state_integral} is
\begin{align}
&\frac{1}{\pi}\int\dx\dy\e^{-\left(x^2 + y^2\right)}\left(x+iy\right)^n)\left(x-iy\right)^m \nonumber \\
&= \frac{1}{\pi} \int \dd{\rho}\rho\dd{\theta}\e^{-\rho^2}\left(\rho\e^{i\theta}\right)^n\left(\rho\e^{-i\theta}\right)^m\nonumber \\
&= \frac{1}{\pi}\underbrace{\int\dd{\theta}\e^{i\theta(n-m)}}_{2\pi\delta_{nm}}\int\dd{\rho}\rho^{n+m+1}\e^{-\rho^2}\nonumber \\
&= 2\delta_{nm}\int\dd{\rho}\rho^{2n+1}\e^{-\rho^2}\nonumber\\ 
&= \delta_{nm}\int_0^\infty\dd{r}r^{-\frac{1}{2}}r^{\frac{2n+1}{2}}e^{-r} = \int_0^\infty\dd{r}r^n\e^{-r} \nonumber\\
&= \delta_{nm}n!,
\end{align}
such that \eqref{eq:completeness_coherent_boson} becomes

\begin{align*}
\frac{1}{2\pi i}\int\dd z \dd{z^*}\e^{-z^*z}\dyad z &= \sum_{n, m}\frac{1}{\sqrt{n!m!}}\dyad{n}{m}\cdot \delta_{nm}n! \\
&= \sum_{n}\dyad{n} = 1.
\end{align*}

Coherent states stays coherent under the propagation of time, but with a different label:

\begin{align*}
\e^{\frac{-iHt}{\hbar}}\ket z &= \e^{\frac{-i\hbar\omega a^\dagger at}{\hbar}}\ket z = \e^{-i\omega ta^\dagger a}\ket z \\
&= \e^{-i\omega ta^\dagger a}\sum_n\frac{z^n}{\sqrt{n!}}\ket n = \sum_n\frac{z^n}{\sqrt{n!}}\e^{-i\omega ta^\dagger a}\ket n \\
&=  \sum_n\frac{z^n}{\sqrt{n!}}\e^{-i\omega tn}\ket n = \sum_n\frac{\left(z\e^{-i\omega t}\right)^n}{\sqrt{n!}}\ket n \\
&= \ket{z\e^{-i\omega t}}
\end{align*}

The propagator in this basis is thus very simple:
\begin{align}
\mel{z_n}{\e^{\frac{-iHt}{\hbar}}}{z_0} &= \braket{z_n}{z_0\e^{-i\omega t}} \\
&= \e^{z_n^*z_0\e^{-i\omega t}}
\end{align}

\subsubsection{The completeness relation for coherent boson states}

\begin{align*}
&\int\left(\prod_\mu\frac{\dd{\varphi_\mu^*}\dd{\varphi_\mu}}{2\pi i}\right)\e^{-\sum_\mu\varphi_\mu^*\varphi_\mu}\dyad{\phi}  \\
&= \int\left(\prod_\mu\frac{\dd{\varphi_\mu^*}\dd{\varphi_\mu}}{2\pi i}\right)\e^{-\sum_\mu\varphi_\mu^*\varphi_\mu}\e^{\sum_\mu\varphi_\mu a_\mu^\dagger}\dyad 0 \e^{-\sum_\mu a_\mu\varphi_\mu^*} \\
&=\int\left(\prod_\mu\frac{\dd{\varphi_\mu^*}\dd{\varphi_\mu}}{2\pi i}\right)\e^{-\sum_\mu\varphi_\mu^*\varphi_\mu} \\
&\cdot \sum_{n_{\mu}=0}^\infty\frac{\varphi_\mu^{n_\mu}}{\sqrt{n_\mu!}}\sum_{n_{\nu}=0}^\infty\frac{\varphi_\nu^{n_\nu}}{\sqrt{n_\nu!}}\cdots\ket{n_\mu, n_\nu, \dots}\\
&\cdot \sum_{m_{\mu}=0}^\infty\frac{\left(\varphi_\mu^*\right)^{m_\mu}}{\sqrt{m_\mu!}}\sum_{m_{\nu}=0}^\infty\frac{\left(\varphi_\nu^*\right)^{m_\nu}}{\sqrt{m_\nu!}}\cdots \bra{m_\mu, m_\nu, \dots} \\
&= \underbrace{\sum_{n_\mu = 0}^\infty\sum_{n_\nu = 0}^\infty\cdots}_{\sum_{\{n_\mu\}}} \dyad{n_\mu, n_\nu, \dots} \\
&= I
\end{align*}


