\section{Coherent states for fermions}

\subsection{Construction}

We will also in the fermionic case make an ansatz on the construction of coherent fermionic states, somewhat similar to \eqref{eq:construction_coherent_boson}:
\begin{align}
\ket \psi &= \e^{-\sum_\mu\xi_\mu c_\mu^\dagger}\ket 0 \\
&= \prod_\mu \left(1-\xi_\mu c_\mu^\dagger\right)\ket 0
\end{align}

It is simpler to show that the ansatz satisfies the definition \eqref{eq:def_fermion_coherent_state} ( \( c_\mu \ket{\psi} = \xi_\mu\ket{\psi}\) ) for fermions than it was for bosons. Use the fact that \(\xi_\mu^2 = 0\) to express the expansion of the exponential function. 
\begin{equation}
c_\mu\prod_\nu\left(1-\xi_\nu c_\nu^\dagger\right)\ket 0 = c_\mu \ket \psi
\end{equation}
affects one of the products:
\begin{align}
c_\mu\left(1-\xi_\mu c_\mu^\dagger\right)\ket 0 &= +\xi_\mu \underbrace{c_\mu c_\mu^\dagger}_{1-c_\mu\dagger c_\mu}\ket 0 \\
&= +\xi_\mu \ket 0  \\
&= \xi_\mu\left(1-\xi_\mu c_\mu^\dagger\right)\ket 0 \\
&\implies \nonumber\\
 &c_\mu\ket \psi = \xi_\mu\ket\psi,
\end{align} 

where we used the anticommutation relations \(\acomm{\xi_\mu}{c_\mu} = \acomm{\xi_\mu}{c_\mu^\dagger} =0\).

\subsection{Properties}

Acting with the creation operator on a coherent fermion state:
\begin{align*}
c_\mu^\dagger\ket\psi &= c_\mu^\dagger\left(1-\xi_\mu c_\mu^\dagger\right)\prod_{\nu \ne \mu}\left(1-\xi_\nu c_\nu^\dagger\right)\ket 0\\
&= -\pdv{\xi_\mu}\left(1-\xi_\mu c_\mu^\dagger\right)\prod_{\nu \ne \mu}\left(1-\xi_\nu c_\nu^\dagger\right)\ket 0 \\
&= -\pdv{\xi_\mu}\ket \psi.
\end{align*}

Similarly, on the ``bra'' vectors:
\begin{align*}
\bra\psi c_\mu &= \prod_{\mu}\bra 0 \left(1+\xi_\mu^*c_\mu\right)c_\mu \\
&=\pdv{\xi_\mu^*}\prod_{\mu}\bra 0 \left(1+\xi_\mu^*c_\mu\right)\\
&= \pdv{\xi_\mu^*}\bra\psi
\end{align*}
NB: Note the plus sign in the product.

The overlap between two coherent fermion states:

\begin{align*}
\braket{\psi}{\psi'} &= \mel{0}{\prod_{\mu, \nu}\left(1+\xi_{\nu}^*c_{\nu}\right)\left(1-\xi_\mu c_\mu^\dagger\right)}{0} \\
&= \prod_{\mu, \nu}\mel{0}{\left(1+\xi_{\nu}^*c_{\nu}\xi_\mu c_\mu^\dagger\right)}{0}\\
&=\prod_{\nu \ne \mu}\cdot 1 \prod_{\mu}\left(1+\xi_\mu^*\xi_\mu\right) \\
&= \prod_{\mu}\left(1+\xi_\mu^*\xi_\mu\right) \\
\text{Re-exponentiation} \implies \braket{\psi}{\psi'} &= \e^{\sum_\mu\xi_\mu^*\xi_\mu}
\end{align*}